LeanYjs/NoCrossOrigin.lean
@@ -1,0 +1,144 @@
+import LeanYjs.Item
+import LeanYjs.ActorId
+import LeanYjs.ItemOriginOrder
+import LeanYjs.ItemOrder
+import LeanYjs.ItemSet
+import LeanYjs.ItemSetInvariant
+import LeanYjs.AntiSymmetry
+
+import Mathlib.Order.Defs.Unbundled
+
+variable {A : Type}
+variable (P : ClosedPredicate A)
+
+theorem no_cross_origin (x y : YjsItem A) :
+  ItemSetInvariant P ->
+  YjsLt' P x y ->
+  YjsLeq' P y.origin x.origin ∨ YjsLeq' P x y.origin := by
+  intros hinv hxy
+  generalize hsize : x.size + y.size = hsize
+  revert x y
+  apply Nat.strongRec' (p := fun hsize => ∀ (x y : YjsItem A),
+    YjsLt' P (YjsPtr.itemPtr x) (YjsPtr.itemPtr y) →
+      x.size + y.size = hsize → YjsLeq' P y.origin x.origin ∨ YjsLeq' P (YjsPtr.itemPtr x) y.origin)
+  intros n ih x y hlt hsize
+  have hpx : P.val x := by
+    apply yjs_lt'_p1; assumption
+  have hpy : P.val y := by
+    apply yjs_lt'_p2; assumption
+  apply yjs_lt'_cases at hlt
+  rcases hlt with
+  ⟨ heqfirst, _ ⟩
+  | ⟨ heqlast, _ ⟩
+  | ⟨ x', hx, hleq' ⟩
+  | ⟨ y', hy, hleq' ⟩
+  | hconflict
+  . cases heqfirst
+  . cases heqlast
+  . cases hx
+    -- apply yjs_leq'_imp_eq_or_yjs_lt' at hleq'
+    obtain ⟨ xo, xr, xid, xc ⟩ := x
+    cases xr with
+    | first =>
+      have ⟨ _, horlt ⟩ := hinv.origin_not_leq _ _ _ _ hpx
+      apply not_ptr_lt_first hinv at horlt
+      cases horlt
+    | last =>
+      simp [YjsItem.rightOrigin] at hleq'
+      have ⟨ _, hleq' ⟩ := hleq'
+      cases hleq' with
+      | inl hleq =>
+        cases hleq
+      | inr hlt' =>
+        apply (not_last_lt_ptr hinv) at hlt'
+        cases hlt'
+    | itemPtr xr =>
+      simp [YjsItem.rightOrigin] at hleq'
+      apply yjs_leq'_imp_eq_or_yjs_lt' at hleq'
+      cases hleq' with
+      | inl hleq =>
+        cases hleq
+        have hreachable : OriginReachable A (YjsPtr.itemPtr (YjsItem.item xo (YjsPtr.itemPtr y) xid xc)) y.origin := by
+          apply @Relation.TransGen.tail (b := YjsPtr.itemPtr y)
+          . apply @Relation.TransGen.single
+            apply OriginReachableStep.reachable_right
+          . obtain ⟨ yo, yr, yid, yc ⟩ := y
+            apply OriginReachableStep.reachable
+        cases hinv.origin_nearest_reachable (x := y.origin) _ _ _ _ hpx hreachable with
+        | inl hleq =>
+          left
+          assumption
+        | inr hleq =>
+          apply yjs_leq'_imp_eq_or_yjs_lt' at hleq
+          cases hleq with
+          | inr hlt =>
+            have hltorigin : YjsLt' P y.origin y := by
+              obtain ⟨ yo, yr, yid, yc ⟩ := y
+              constructor; apply YjsLt.ltOriginOrder <;> try assumption
+              . apply P.property.closedLeft; assumption
+              . apply OriginLt.lt_left
+            cases yjs_lt_anti_symm hinv y.origin y hltorigin hlt
+          | inl heq =>
+            obtain ⟨ yo, yr, yid, yc ⟩ := y
+            simp [YjsItem.origin] at heq
+            cases heq
+      | inr hlt =>
+        have hsize' : xr.size + y.size < n := by
+          simp [YjsPtr.size, YjsItem.size] at hsize
+          omega
+        cases ih (xr.size + y.size) hsize' xr y hlt (by simp) with
+        | inl hleq =>
+          obtain ⟨ h, hleq ⟩ := hleq
+          left
+          have hreachable : OriginReachable A (YjsPtr.itemPtr (YjsItem.item xo xr xid xc)) xr.origin := by
+            apply Relation.TransGen.tail
+            apply Relation.TransGen.single
+            apply OriginReachableStep.reachable_right
+            obtain ⟨ xro, xrr, xrid, xrc ⟩ := xr
+            apply OriginReachableStep.reachable
+          have ⟨ _, hlt ⟩ : YjsLeq' P xr.origin xo := by
+            cases hinv.origin_nearest_reachable _ _ _ _ _ hpx hreachable with
+            | inl hleq => assumption
+            | inr hleq =>
+              have hlt : YjsLt' P xr.origin xr := by
+                obtain ⟨ xro, xrr, xrid, xrc ⟩ := xr
+                constructor; apply YjsLt.ltOriginOrder <;> try assumption
+                . apply P.property.closedLeft
+                  apply P.property.closedRight
+                  assumption
+                . apply P.property.closedRight
+                  assumption
+                apply OriginLt.lt_left
+              apply yjs_leq'_imp_eq_or_yjs_lt' at hleq
+              cases hleq with
+              | inl heq =>
+                rw [heq] at hlt
+                cases yjs_lt_anti_symm hinv _ _ hlt hlt
+              | inr hlt' =>
+                cases yjs_lt_anti_symm hinv _ _ hlt hlt'
+          apply yjs_leq_p_trans hinv _ _ _ _ _ hleq
+          assumption
+        | inr hlt =>
+          obtain ⟨ _, hlt ⟩ := hlt
+          right
+          have ⟨ _, hlt' ⟩ : YjsLt' P (YjsPtr.itemPtr (YjsItem.item xo (YjsPtr.itemPtr xr) xid xc)) xr := by
+            constructor; apply YjsLt.ltOriginOrder <;> try assumption
+            . apply P.property.closedRight; assumption
+            . apply OriginLt.lt_right
+          apply yjs_leq_p_trans (inv := hinv) (y := xr) <;> try assumption
+          right
+          assumption
+  . cases hy
+    right; assumption
+  . obtain ⟨ _, hconflict ⟩ := hconflict
+    cases hconflict with
+    | ltOriginDiff =>
+      left
+      constructor
+      right
+      assumption
+    | ltOriginSame =>
+      left
+      exists 0
+      left
+      eq_refl
